feat: solve `tr` goals using local optimization
This commit also includes various fixes to the things added in the
previous commits and some unexpected breaking test cases (which was not
manifested due to the fallback to the old `veil_solve_tr`).

Veil/Frontend/DSL/Module/Names.lean
@@ -157,4 +157,9 @@ def localMeetsSpecificationIfSuccessfulAssumingName : Name :=
 def localMeetsSpecificationIfSuccessfulAssuming : Ident :=
   mkIdent localMeetsSpecificationIfSuccessfulAssumingName
 
+def localTransitionMeetsSpecificationIfSuccessfulAssumingName : Name :=
+  mkVeilImplementationDetailName `transition_meetsSpecificationIfSuccessfulAssuming_local
+def localTransitionMeetsSpecificationIfSuccessfulAssuming : Ident :=
+  mkIdent localTransitionMeetsSpecificationIfSuccessfulAssumingName
+
 end Veil
