Veil/Frontend/DSL/Module/Elaborators.lean
@@ -299,6 +299,11 @@ def Module.ensureSpecIsFinalized (mod : Module) (stx : Syntax) : CommandElabM Mo
           elabVeilCommand localMeetsCmd
         catch ex =>
           logWarningAt invariantCmd m!"unable to define {localMeetsSpecificationIfSuccessfulAssumingName}: {ex.toMessageData}"
+        try
+          let localTrMeetsCmd ← liftTermElabM mod.defineTransitionMeetsSpecificationIfSuccessfulAssumingLocalTheorem
+          elabVeilCommand localTrMeetsCmd
+        catch ex =>
+          logWarningAt invariantCmd m!"unable to define {localTransitionMeetsSpecificationIfSuccessfulAssumingName}: {ex.toMessageData}"
       return mod
     let mod ← withTraceNode `veil.perf.elaborator.decl.Safeties (fun _ => return "Safeties") do
       let (safetyCmd, mod) ← mod.assembleSafeties
